src/voteprivacy/auxDefs.v
@@ -9,7 +9,8 @@ Require Import List.
 Import ListNotations.
 
 Section auxProps.
-  Axiom ifMorphPair: forall b t1 t2 t3, (t1, If b then t2 else t3) # If b then (t1, t2) else (t1, t3).
+  Axiom ifMorphPair2: forall b t1 t2 t3, (t1, If b then t2 else t3) # If b then (t1, t2) else (t1, t3).
+  Axiom ifMorphPair1: forall b t1 t2 t3, (If b then t1 else t2, t3) # If b then (t1, t3) else (t2, t3).
   Axiom andB_elim: forall b1 b2 t1 t2, (If b1 & b2 then t1 else t2) # (If b1 then (If b2 then t1 else t2) else t2).
   Axiom ifMorphIfThen: forall b1 b2 t1 t2 t3, (If b1 then (If b2 then t1 else t2) else t3) # (If b2 then (If b1 then t1 else t3) else (If b1 then t2 else t3)).
   Axiom orB_FAlse_r: forall b, b or FAlse = b.
